EasyCrypt/SimpleORAMExtra.ec
@@ -1,0 +1,9 @@
+require import SimpleORAM.
+
+
+lemma EC_security :
+  equiv[
+    SimpleORAM.ORAM.compile ~ SimpleORAM.ORAM.compile :
+      true ==> SimpleORAM.ORAM.leakage{1} = SimpleORAM.ORAM.leakage{2}
+  ].
+admitted.
